\graphicspath{}
\begin{highlight}{Spezielle Grenzwerte von Folgen}
    \tcbsubtitle{$n \to \infty$}
    \begin{equation*}
        n^x q^n \to 0 \quad \forall x \in \Z~\text{und}~0 \leq q \leq 1
    \end{equation*}
    \begin{equation*}
         n(\sqrt[n]{x} - 1) \to \ln x \quad \forall x>0
    \end{equation*}
    \begin{equation*}
        \sqrt[n]{a_n} \to 1 ~\text{wenn}~ \lim_{n \to \infty} a_n > 0 ~\text{und}~ \forall a_n > 0 
    \end{equation*}
    \begin{center}
        \begin{minipage}{0.3\linewidth}
            \begin{align*}
                \frac{1}{n} &\to 0\\
                1 + \frac{1}{n} &\to 1\\
                \frac{2n}{2^n} &\to 0\\
                \sqrt[n]{n} = n^{\frac{1}{n}} &\to 1\\
                \sqrt[n]{n!} &\to \infty\\
                \frac{1}{n}\sqrt[n]{n!} &\to \frac{1}{e}\\
                \frac{x^n}{n!} &\to 0\\
                \frac{n^n}{n!} &\to \infty
            \end{align*}
        \end{minipage}
        \hfill\vline\hfill
        \begin{minipage}{0.3\linewidth}
            \begin{align*}
                % \frac{a^n}{n!} &\to 0\\
                % \left(\frac{n+1}{n}\right)^n &\to e\\
                e^n &\to \infty\\
                e^{-n} &\to 0\\
                \frac{e^n}{n^x} &\to \infty\\
                \frac{\sin n}{n} &\to 0\\
                \arctan n &\to \frac{\pi}{2}\\
                ln(n) &\to \infty\\
                \frac{ln(n)}{n} &\to 0\\
                \frac{log(n)}{n - 1} &\to 1
            \end{align*}
        \end{minipage}
        \hfill\vline\hfill
        \begin{minipage}{0.3\linewidth}
            \begin{align*}
                \forall k \in \Q^+ \hspace{2mm}\frac{1}{n^k} &\to 0\\
                \left(1 + n\right)^{\frac{1}{n}} &\to 1\\
                \left(1 + \frac{1}{n}\right)^x &\to 1\\
                \left(1 + \frac{1}{n}\right)^n &\to e\\
                \left(1 + \frac{x}{n}\right)^n &\to e^x\\
                \left(1 - \frac{1}{n}\right)^n &\to \frac{1}{e}\\
                \left(\frac{n}{n + x}\right)^n &\to e^{-x}
                % \left(1 - \frac{x}{n}\right)^n &\to e^{-x}\\
                % \binom{a}{n} &\to 0 \quad\text{fÃ¼r}~a > -1
            \end{align*}
        \end{minipage}
    \end{center}
    \begin{comment}
    \tcbsubtitle{$n \to 0$}
     \begin{minipage}{0.3\linewidth}
        \begin{align*}
            \ln n &\to -\infty\\
            \frac{ln(n+1)}{n} &\to 1\\
            n \log n &\to 0\\
            \frac{\log 1 - n}{n} &\to -1\\
            \frac{\log 1 - n}{n} &\to -1\\
            \forall x>0 \hspace{1mm}\frac{x^n-1}{n} &\to \ln(x)
        \end{align*}
    \end{minipage}
    \hfill\vline\hfill
    \begin{minipage}{0.3\linewidth}
        \begin{align*}
            \frac{\sin n}{n} &\to 1\\
            \frac{\cos n - 1}{n} &\to 0\\
            \frac{1}{\cos n} &\to 1\\
            \frac{1 - \cos n}{n^2} &\to \frac{1}{2}
        \end{align*}
    \end{minipage}
    \hfill\vline\hfill
    \begin{minipage}{0.3\linewidth}
        \begin{align*}
            \frac{1}{\arctan n} &\to 1\\
            \frac{e^n - 1}{n} &\to 1\\
            \frac{e^an - 1}{n} &\to a\\
            \left(1 + n\right)^{\frac{1}{n}} &\to e
        \end{align*}
    \end{minipage}
    \tcbsubtitle{Weitere Grenzwerte}
     \begin{minipage}{0.3\linewidth}
        \emph{$n \to -\infty$}
        \begin{align*}
            e^n &\to 0\\
            e^{-n} &\to \infty\\
            ne^n &\to 0
        \end{align*}
        \emph{$n \to 0+$}
        \begin{align*}
            n \ln n &\to 0
        \end{align*}
    \end{minipage}
    \hfill\vline\hfill
    \begin{minipage}{0.3\linewidth}
        \emph{$n \to \pm\infty$}
        \begin{align*}
            \left(1 + \frac{1}{n}\right)^n &\to e\\
            \left(1 + \frac{x}{n}\right)^an &\to e^ax
        \end{align*}
    \end{minipage}
    \hfill\vline\hfill
    \begin{minipage}{0.3\linewidth}
    \emph{$n \to \frac{\pi-}{2}$}
        \begin{align*}
            \tan x &\to +\infty
        \end{align*}
    \emph{$n \to \frac{\pi+}{2}$}
        \begin{align*}
            \tan x &\to -\infty
        \end{align*}
    \end{minipage}
    \end{comment}
    \tcbsubtitle{Divergente Folgen}
    \begin{align*}
        &a_{n}=(-1)^{n}=(-1,1,-1,1,-1 \ldots) \\
        &a_{n}=3+2 n=(5,7,9,11, \ldots)
    \end{align*}
\end{highlight}


