\begin{example}
	Gib eine Formel f√ºr $1^4 + 2^4 + 3^4 + \ldots n^4$ an\\
	Verwende Allgemeine Formel und $B_0 = 1$, $B_1 = - \frac{1}{2}$, $B_2 = \frac{1}{6}$, $B_3 = 0$, $B_4 = -\frac{1}{30}$\\ \\
    $1^l + 2^l + \ldots + n^l = \frac{1}{l+1} \sum^{l}_{j=0} (-1)^j \begin{pmatrix}l+1\\j\end{pmatrix} B_j n^{l+1-j}\\
					 = \frac{1}{5} \sum^{4}_{j=0} \begin{pmatrix}5\\j\end{pmatrix} B_j \cdot (-1)^j n^{5-j}\\
					 = \frac{1}{5} \left( B_0 n^5 - \frac{5!}{4!} B_1 n^4 + \frac{5!}{3!2!} B_2 n^3 -0 + \frac{5!}{4!} B_4 n \right)\\
					 = \frac{1}{5} \left( n^5 - \frac{5}{2} n^4 + \frac{5}{3} n^3 - \frac{1}{6} n \right)$
\end{example}