\subsubsection{Grundlegende Ableitungen}
\begin{iequation}
    \def\arraystretch{1.8}
    \begin{array}{c|c|c}
        \od{}{x} 1 = 0 & \od{}{x} x = 1 & \od{}{x} x^a = a\cdot x^{a-1}\\
        \hline
        \od{}{x} e^{a x} = a\cdot e^{ax} & \od{}{x} a^x = a^x \cdot \ln(a) & \od{}{x} \ln (x) = \frac{1}{x}\\
        \hline
        \od{}{x} \log_a (x) = \frac{1}{x \cdot \ln(a)} & \od{}{x}\sin(x) = \cos(x) & \od{}{x}\cos(x) = -\sin(x)\\
    \end{array}
\end{iequation}
\begin{iequation}
    \def\arraystretch{1.8}
    \begin{array}{c|c}
        \od{}{x} \arcsin(x) = \frac{1}{\sqrt{1-x^2}} & \od{}{x} \arccos(x) = \frac{-1}{\sqrt{1-x^2}}\\
        \hline
	\od{}{x} \arctan(x) = \frac{1}{x^2+1} & \od{}{x} \tan(x) = \frac{1}{\cos^2(x)}=1+\tan^2(x)\\
    \end{array}
\end{iequation}
\subsubsection{GÃ¤ngige Ableitungen}
\begin{equation*}
    \def\arraystretch{1.8}
    \begin{array}{c|c}
        \od{}{x} \frac{1}{x^n}=\frac{-n}{x^{n+1}} & \od{}{x} \sqrt[n]{x}=\frac{1}{n\sqrt[n]{x^{n-1}}}\\
        \hline
        \od{}{x} x^x = x^x(1+\ln x) & \od{}{x} \log_ax = \frac{1}{x}\frac{1}{\ln x}\\
        \hline
        \od{}{x} \exp(\exp(x)) = \exp(\exp(x) + x) & \od{}{x} \cot (x) = -\frac{1}{\sin^2(x)} = -1 - \cot^2(x)\\
        \hline
        % \od{}{x} \arcsin(x) = \frac{1}{\sqrt{1-x^2}} & \od{}{x} \arccos(x) = \frac{-1}{\sqrt{1-x^2}}\\
        % \hline
        % \od{}{x} \arctan(x) = \frac{1}{x^2+1} & \\
        % \hline
        \od{}{x} \sinh(x) = \cosh(x) & \od{}{x} \cosh(x) = \sinh(x)\\
	\hline
	\od{}{x} |x| = \sgn (x) \quad x \neq 0 &
    \end{array}
\end{equation*}
\raggedcolumns
\columnbreak