\begin{example}
	Berechne $\int \frac{x+1}{x^3 + x^2 - 6x} \dif x$ mittels PBZ.
	\begin{gather*}
		\frac{x+1}{x^3 + x^2 - 6x} = \frac{x+1}{x(x-2)(x+3)} = \frac{A}{x} + \frac{B}{x-2} + \frac{C}{x+3}\\
		\Rightarrow A + B + C = 0 \quad A + 3B - 2C = 1 \quad -6A = 1
	\end{gather*}
	Daraus folgt: $A = -\frac{1}{6}$, $B = \frac{3}{10}$, $C = -\frac{2}{15}$
	\begin{align*}
		\int \frac{x+1}{x^3 + x^2 - 6x} \dif x &= -\frac{1}{6} \int \frac{1}{x} \dif x + \frac{3}{10} \int \frac{1}{x-2} \dif x - \frac{2}{15} \int \frac{1}{x+3} \dif x\\
						       &= -\frac{1}{6} \log |x| + \frac{3}{10} \log |x-2| - \frac{2}{5} \log |x+3| + C 
	\end{align*}
\end{example}